renamed file. finished proof of queue client. clean up needed. tasks updated from feedback.

theories/queue_client.v
@@ -2,7 +2,6 @@ From iris.algebra Require Import list agree lib.frac_auth.
 From iris.heap_lang Require Import lang proofmode notation spawn.
 From iris.base_logic.lib Require Import invariants token.
 From MSQueue Require Import queue_specs.
-From MSQueue Require Import lockFreeMSQ_impl.
 
 Section client.
 
@@ -27,27 +26,26 @@ Definition enqdeq : val :=
 
 Definition queueAdd : val :=
   λ: "a" "b",
-    let: "v_q" := queue_specs.initialize #() in
+    let: "v_q" := initialize #() in
     let: "j" := spawn (λ: <>, enqdeq "v_q" "a") in
     let: "x" := enqdeq "v_q" "b" in
     let: "y" := spawn.join "j" in
     "x" + "y".
 
-
 Variable Ns: namespace.
 Notation Nqa := (N .@ "QueueAdd").
 
-Record QAddgnames := {  γ_D1     : gname;
-                        γ_D2     : gname;
-                        γ_A      : gname;
-                        γ_B      : gname;
-                      }.
+Record QAgnames := {  γ_D1     : gname;
+                      γ_D2     : gname;
+                      γ_A      : gname;
+                      γ_B      : gname;
+                    }.
 
 (* ----- Tokens ----- *)
-Definition TokD1 (g : QAddgnames) := token g.(γ_D1).
-Definition TokD2 (g : QAddgnames) := token g.(γ_D2).
-Definition TokA (g : QAddgnames) := token g.(γ_A).
-Definition TokB (g : QAddgnames) := token g.(γ_B).
+Definition TokD1 (g : QAgnames) := token g.(γ_D1).
+Definition TokD2 (g : QAgnames) := token g.(γ_D2).
+Definition TokA (g : QAgnames) := token g.(γ_A).
+Definition TokB (g : QAgnames) := token g.(γ_B).
 
 Definition contentsInv G Ga a b : iProp Σ :=
   (γ_Abst G) ⤇◯ [] ∗ TokD1 Ga ∗ TokD2 Ga ∨
@@ -56,24 +54,20 @@ Definition contentsInv G Ga a b : iProp Σ :=
   (γ_Abst G) ⤇◯ [a; b] ∗ TokA Ga ∗ TokB Ga ∨
   (γ_Abst G) ⤇◯ [b; a] ∗ TokB Ga ∗ TokA Ga.
 
-Definition enqdeq_post v a b Ga : iProp Σ := ⌜v = #a⌝ ∗ TokA Ga ∨ ⌜v = #b⌝ ∗ TokB Ga.
+Definition case_a_b v a b Ga : iProp Σ := ⌜v = #a⌝ ∗ TokA Ga ∨ ⌜v = #b⌝ ∗ TokB Ga.
 
 Lemma enqdeq_spec : ∀(a b c : Z) Ga G (v_q : val),
   {{{ isQueue v_q G ∗ inv Nqa (contentsInv G Ga #a #b) ∗
               ((TokA Ga ∗ ⌜c = a⌝) ∨ (TokB Ga ∗ ⌜c = b⌝)) }}}
     enqdeq v_q #c
-  {{{v, RET v; enqdeq_post v a b Ga }}}.
+  {{{v, RET v; case_a_b v a b Ga }}}.
 Proof.
   iIntros (a b c Ga G v_q Φ) "(#HisQueue & #Hinv & Hcase) HΦ".
   wp_lam.
   wp_pures.
   set (P := ((TokA Ga ∗ ⌜c = a⌝) ∨ (TokB Ga ∗ ⌜c = b⌝))%I).
   set (Q := (TokD1 Ga ∨ TokD2 Ga)%I).
-  (* TODO: find out how to apply enqueue spec *)
-  (* wp_apply (enqueue_spec v_q #c G P Q with "[] [Hcase]"). *)
-  iAssert (□(∀xs_v, (γ_Abst G ⤇● xs_v ∗ P ={⊤ ∖ ↑Ni}=∗ ▷ (γ_Abst G ⤇● (#c :: xs_v) ∗ Q))) -∗ {{{ isQueue v_q G ∗ P}}} enqueue v_q #c {{{ w, RET w; Q }}})%I as "Henqspec".
-  { admit. }
-  wp_apply ("Henqspec" with "[] [Hcase]"); iClear "Henqspec". (* TODO: REMOVE*)
+  wp_apply (enqueue_spec v_q #c G P Q with "[] [Hcase]").
   (* Proving viewshift *)
   {
     iModIntro.
@@ -94,20 +88,14 @@ Proof.
     | iMod (queue_contents_update _ _ _ [ #b ] with "Hauth Hfrag") as "[Hauth Hfrag]"
     | iMod (queue_contents_update _ _ _ [ #b ; #a ] with "Hauth Hfrag") as "[Hauth Hfrag]"
     | iMod (queue_contents_update _ _ _ [ #a ; #b ] with "Hauth Hfrag") as "[Hauth Hfrag]" ];
-    iModIntro.
+    iModIntro;
+    unfold contentsInv;
     (* Close the invariant in the updated state *)
-    + iSplitL "HTokA' HTokD1 Hfrag". (* Can give up either D1 or D2 *)
-      { iNext. iRight. iLeft. iFrame. }
-      by iFrame.
-    + iSplitL "HTokB' HTokD1 Hfrag". (* Can give up either D1 or D2 *)
-      { iNext. iRight. iRight. iLeft. iFrame. }
-      by iFrame.
-    + iSplitL "HTokA HTokB' Hfrag".
-      { iNext. iRight. iRight. iRight. iRight. iFrame. }
-      by iFrame.
-    + iSplitL "HTokA' HTokB Hfrag".
-      { iNext. iRight. iRight. iRight. iLeft. iFrame. }
-      by iFrame.
+    [ iSplitL "HTokA' HTokD1 Hfrag" (* Can give up either D1 or D2 *)
+    | iSplitL "HTokB' HTokD1 Hfrag" (* Can give up either D1 or D2 *)
+    | iSplitL "HTokA HTokB' Hfrag"
+    | iSplitL "HTokA' HTokB Hfrag" ];
+    eauto 6 with iFrame.
   }
   (* Proving pre-condition of hocap enqueue spec *)
   { by iFrame. }
@@ -117,20 +105,7 @@ Proof.
   wp_bind (dequeue v_q).
   set (P' := Q%I : iProp Σ).
   set (Q' := λ w, (⌜w = SOMEV #a⌝ ∗ TokA Ga ∨ ⌜w = SOMEV #b⌝ ∗ TokB Ga)%I : iProp Σ).
-  (* TODO: find out how to apply dequeue spec *)
-  (* wp_apply (dequeue_spec v_q G P Q'). *)
-  iAssert (□(∀xs_v, (γ_Abst G ⤇● xs_v ∗ P'
-            ={⊤ ∖ ↑Ni}=∗
-            ▷ (( ⌜xs_v = []⌝ ∗ γ_Abst G ⤇● xs_v ∗ Q' NONEV) ∨
-            (∃v xs_v', ⌜xs_v = xs_v' ++ [v]⌝ ∗ γ_Abst G ⤇● xs_v' ∗ Q' (SOMEV v)))
-          )
-          )
-          -∗
-          {{{ isQueue v_q G ∗ P' }}}
-            dequeue v_q
-          {{{ w, RET w; Q' w }}})%I as "Hdeqspec".
-  { admit. }
-  wp_apply ("Hdeqspec" with "[] [HQ]"); iClear "Hdeqspec". (* TODO: REMOVE *)
+  wp_apply (dequeue_spec v_q G P' Q' with "[] [HQ]").
   (* Proving viewshift *)
   {
     iModIntro.
@@ -156,32 +131,17 @@ Proof.
     | iMod (queue_contents_update _ _ _ [ #b ] with "Hauth Hfrag") as "[Hauth Hfrag]" ];
     iModIntro;
     iFrame "Hauth";
-    unfold Q'.
+    unfold Q', contentsInv;
     (* Close the invariant in the updated state *)
-    + iSplitL "HTokD1 HTokD2' Hfrag".
-      { iNext. iLeft. iFrame. }
-      eauto 7.
-    + iSplitL "HTokD1' HTokD2 Hfrag".
-      { iNext. iLeft. iFrame. }
-      eauto 7.
-    + iSplitL "HTokD1 HTokD2' Hfrag".
-      { iNext. iLeft. iFrame. }
-      eauto 7.
-    + iSplitL "HTokD1' HTokD2 Hfrag".
-      { iNext. iLeft. iFrame. }
-      eauto 7.
-    + iSplitL "HTokD1' HTokA Hfrag".
-      { iNext. iRight. iLeft. iFrame. }
-      eauto 7.
-    + iSplitL "HTokD2' HTokA Hfrag".
-      { iNext. iRight. iLeft. iFrame. }
-      eauto 7.
-    + iSplitL "HTokD1' HTokB Hfrag".
-      { iNext. iRight. iRight. iLeft. iFrame. }
-      eauto 7.
-    + iSplitL "HTokD2' HTokB Hfrag".
-      { iNext. iRight. iRight. iLeft. iFrame. }
-      eauto 7.
+    [ iSplitL "HTokD1 HTokD2' Hfrag"
+    | iSplitL "HTokD1' HTokD2 Hfrag"
+    | iSplitL "HTokD1 HTokD2' Hfrag"
+    | iSplitL "HTokD1' HTokD2 Hfrag"
+    | iSplitL "HTokD1' HTokA Hfrag"
+    | iSplitL "HTokD2' HTokA Hfrag"
+    | iSplitL "HTokD1' HTokB Hfrag"
+    | iSplitL "HTokD2' HTokB Hfrag" ];
+    eauto 7 with iFrame.
   }
   (* Proving pre-condition of hocap dequeue spec *)
   { by iFrame. }
@@ -191,7 +151,7 @@ Proof.
   iApply "HΦ";
   [iLeft | iRight];
   by iFrame.
-Admitted.
+Qed.
 
 Lemma queueAdd_spec : ∀(a b : Z),
   {{{ True }}} queueAdd #a #b {{{v, RET v; ⌜v = #(a + b)⌝}}}.
@@ -213,19 +173,19 @@ Proof.
   iMod (inv_alloc Nqa _ (contentsInv G Ga #a #b) with "[Hγ_D1 Hγ_D2 Hfrag]") as "#HqaInv".
   { iNext. iLeft. iFrame. }
   wp_pures.
-  wp_apply (spawn_spec Ns (λ v, enqdeq_post v a b Ga) _ with "[Hγ_A]").
+  wp_apply (spawn_spec Ns (λ v, case_a_b v a b Ga) _ with "[Hγ_A]").
   - wp_lam.
     wp_apply (enqdeq_spec a b a Ga G v_q with "[HisQueue Hγ_A]"); auto.
   - iIntros (jloc) "Hjhandle".
     wp_pures.
     wp_apply (enqdeq_spec a b b Ga G v_q with "[Hγ_B]"); first iFrame "#"; auto.
-    iIntros (x) "Hor".
+    iIntros (x) "Hcase".
     wp_pures.
     wp_apply (join_spec with "Hjhandle").
-    iIntros (y) "Hor'".
+    iIntros (y) "Hcase'".
     wp_pures.
-    iDestruct "Hor" as "[[-> HTokA]|[-> HTokB]]";
-    iDestruct "Hor'" as "[[-> HTokA']|[-> HTokB']]"; 
+    iDestruct "Hcase" as "[[-> HTokA]|[-> HTokB]]";
+    iDestruct "Hcase'" as "[[-> HTokA']|[-> HTokB']]"; 
     [ by iCombine "HTokA HTokA'" gives "%Hcontra" | |
     | by iCombine "HTokB HTokB'" gives "%Hcontra" ];
     wp_pures;
@@ -233,3 +193,5 @@ Proof.
     iApply "HΦ"; first done.
     by rewrite Z.add_comm.
 Qed.
+
+End client.
